theories/Syntax/Stmt.v
@@ -1,6 +1,6 @@
-From stdpp Require Import base gmap.
 From Metaconfigurations Require Import Syntax.Term Object.
 Require Import Coq.Strings.String.
+From stdpp Require Import base gmap.
 
 Section Stmt.
 
@@ -29,3 +29,24 @@ Arguments Goto {_ _ _ _}.
 Arguments Return {_ _ _ _}.
 Arguments Invoke {_ _ _ _}.
 Arguments Skip {_ _ _ _}.
+
+(** [free x s] is provable iff variable [x] is free in statement [s] *)
+Inductive free {Π Ω} `{Object Π Ω} : string → t Π Ω → Prop :=
+  | free_seq_l x s₁ s₂ : free x s₁ → free x (Seq s₁ s₂)
+  | free_seq_r x s₁ s₂ : free x s₂ → free x (Seq s₁ s₂)
+  | free_assign x e y : x ≠ y → Term.free y e → free y (Assign x e)
+  | free_if_guard x e s₁ s₂ : Term.free x e → free x (If e s₁ s₂)
+  | free_if_l x e s₁ s₂ : free x s₁ → free x (If e s₁ s₂)
+  | free_if_r x e s₁ s₂ : free x s₂ → free x (If e s₁ s₂)
+  | free_return x e : Term.free x e → free x (Return e).
+
+Instance subst_stmt {Π Ω} `{Object Π Ω} : Subst (t Π Ω) :=
+  fix subst_stmt eₓ x s :=
+    match s with
+    | Seq s₁ s₂ => Seq (subst_stmt eₓ x s₁) (subst_stmt eₓ x s₂)
+    | Assign x e => Assign x (subst eₓ x e)
+    | If e s₁ s₂ => If (subst eₓ x e) (subst_stmt eₓ x s₁) (subst_stmt eₓ x s₁)
+    | Return e => Return (subst eₓ x e)
+    | Invoke (Invocation ω op e) => Invoke (Invocation ω op (subst eₓ x e))
+    | Goto _ | Skip => s
+    end.
